theories/Combi/ordtree.v
@@ -1,0 +1,275 @@
+(** * Combi.Combi.ordree : Ordered Trees *)
+(******************************************************************************)
+(*      Copyright (C) 2014-2018 Florent Hivert <florent.hivert@lri.fr>        *)
+(*                                                                            *)
+(*  Distributed under the terms of the GNU General Public License (GPL)       *)
+(*                                                                            *)
+(*    This code is distributed in the hope that it will be useful,            *)
+(*    but WITHOUT ANY WARRANTY; without even the implied warranty of          *)
+(*    MERCHANTABILITY or FITNESS FOR A PARTICULAR PURPOSE.  See the GNU       *)
+(*    General Public License for more details.                                *)
+(*                                                                            *)
+(*  The full text of the GPL is available at:                                 *)
+(*                                                                            *)
+(*                  http://www.gnu.org/licenses/                              *)
+(******************************************************************************)
+(** * Ordered Trees
+
+An _ordered tree_ is a rooted tree such that each node has a possibly empty
+list of child that are ordered trees.
+
+Basic definitions:
+
+- [ordtree]   == the type of ordered trees. This is canonically a [countType]
+- [forest]    == the type of forest, that is sequence of ordered trees
+- [OrdNode f] == the ordered tree with subtrees from the forest [f]
+
+Ordered trees of size n:
+
+- [size_ordtree t]   == the number of node of the ordered tree [t]
+- [enum_ordtreesz n] == the list of a ordered trees of size [n]
+- [ordtreesz n]      == the Sigma type for ordered trees of size [n].
+        This is canonically a [finType] with enumeration [enum_ordtreesz n]
+- [depth_ordtree t]  == the depth of the ordered tree [t], that is the
+        maximum number of node on a branch.
+
+ *********************)
+From HB Require Import structures.
+From mathcomp Require Import all_boot.
+Require Import tools combclass bintree.
+
+Set SsrOldRewriteGoalsOrder.  (* change to Unset and remove the line when requiring MathComp >= 2.6 *)
+Set Implicit Arguments.
+Unset Strict Implicit.
+Unset Printing Implicit Defensive.
+
+
+(** * Inductive type for ordered trees *)
+Unset Elimination Schemes.
+Inductive ordtree : Set := OrdNode : seq ordtree -> ordtree.
+Set Elimination Schemes.
+Notation forest := (seq ordtree).
+
+Lemma OrdNode_inj : injective OrdNode.
+Proof. by move=> f1 f2 []. Qed.
+
+(** Induction scheme for ordtrees *)
+Section Recursion.
+
+Variables (P : ordtree -> Type) (PF : seq ordtree -> Type).
+Hypothesis HPnil : PF [::].
+Hypothesis IHforest : forall tr f, P tr -> PF f -> PF (tr :: f).
+Hypothesis IHtree : forall f, PF f -> P (OrdNode f).
+
+Fixpoint recforest rt f : PF f :=
+  if f is tr :: tlf then IHforest (rt tr) (recforest rt tlf)
+  else HPnil.
+Fixpoint rectree t : P t :=
+  let: OrdNode f := t in IHtree (recforest rectree f).
+
+End Recursion.
+Definition indtreeforest
+  (P : ordtree -> Prop) (PF : forest -> Prop) := @rectree P PF.
+
+
+Fixpoint eq_forest (eqtr : ordtree -> ordtree -> bool) (f1 f2 : seq ordtree) :=
+  match f1, f2 with
+  | [::], [::] => true
+  | tr1 :: tl1, tr2 :: tl2 => eqtr tr1 tr2 && eq_forest eqtr tl1 tl2
+  | _, _ => false
+  end.
+Fixpoint eq_ordtree tr1 tr2 :=
+  match tr1, tr2 with
+    OrdNode f1, OrdNode f2 => eq_forest eq_ordtree f1 f2
+  end.
+Fact eq_ordtreeP : Equality.axiom eq_ordtree.
+Proof.
+move=> t1 t2; apply: (iffP idP) => [|<-]; first last.
+  by apply: (indtreeforest
+               (P := fun t => eq_ordtree t t)
+               (PF := fun f => eq_forest eq_ordtree f f)) => //= tr f -> ->.
+apply: (indtreeforest
+          (P := fun t => forall t2, eq_ordtree t t2 -> t = t2)
+          (PF := fun f => forall f2, eq_forest eq_ordtree f f2 -> f = f2))
+     => {t1 t2}.
+- by case.
+- by move=> tr f IHt IHf /=; case=> [|t2 f2] // /andP[/IHt-> /IHf->].
+- by move=> f IHf [f2] /= /IHf ->.
+Qed.
+HB.instance Definition _ := hasDecEq.Build ordtree eq_ordtreeP.
+
+
+Section SimpleRecursion.
+
+Variables (P : ordtree -> Type).
+Hypothesis IHtree :
+  forall f : forest, (forall t : ordtree, t \in f -> P t) -> P (OrdNode f).
+Lemma rec_tree t : P t.
+Proof.
+apply (rectree (PF := fun f => forall t : ordtree, t \in f -> P t))
+      => // tr f Htr Hf tr1.
+by rewrite inE; case: eqP => [-> // | _ /= /Hf].
+Qed.
+
+End SimpleRecursion.
+Definition indtree (P : ordtree -> Prop) := @rec_tree P.
+
+
+Fixpoint ord_to_bintree (t : ordtree) : bintree :=
+  let fix f_to_bin t_to_bin (f : forest) : bintree :=
+    match f with
+    | [::] => BinLeaf
+    | t :: ftl => BinNode (t_to_bin t) (f_to_bin t_to_bin ftl)
+    end
+  in let: OrdNode f := t in f_to_bin ord_to_bintree f.
+Definition forest_to_bintree f := ord_to_bintree (OrdNode f).
+
+Fixpoint bin_to_forest (t : bintree) : forest :=
+  if t is BinNode l r then OrdNode (bin_to_forest l) :: bin_to_forest r
+  else [::].
+Definition bin_to_ordtree t := OrdNode (bin_to_forest t).
+
+Lemma bin_to_forestK : cancel bin_to_forest forest_to_bintree.
+Proof. by rewrite /forest_to_bintree /=; elim=> [| l /[swap] r /= -> ->]. Qed.
+Lemma bin_to_ordtreeK : cancel bin_to_ordtree ord_to_bintree.
+Proof. exact: bin_to_forestK. Qed.
+
+Lemma ord_to_bintreeK : cancel ord_to_bintree bin_to_ordtree.
+Proof.
+rewrite /bin_to_ordtree; elim/indtree; elim => [// | t f IHf IHt /=].
+congr (OrdNode (_ :: _)); first by apply: IHt; rewrite inE eqxx.
+by apply/OrdNode_inj/IHf => t0 t0inf; apply: IHt; rewrite inE t0inf orbT.
+Qed.
+Lemma forest_to_bintreeK : cancel forest_to_bintree bin_to_forest.
+Proof. by move=> f; apply OrdNode_inj; exact: ord_to_bintreeK. Qed.
+
+HB.instance Definition _ :=
+  Choice.copy ordtree (can_type ord_to_bintreeK).
+HB.instance Definition _ :=
+  Countable.copy ordtree (can_type ord_to_bintreeK).
+
+
+Fixpoint size_ordtree t :=
+  let: OrdNode f := t in (sumn [seq size_ordtree t | t <- f]).+1.
+Lemma size_ordtreeE f :
+  size_ordtree (OrdNode f) = (sumn [seq size_ordtree t | t <- f]).+1.
+Proof. by []. Qed.
+Lemma size_ordtree_pos t : size_ordtree t > 0.
+Proof. by case: t. Qed.
+Lemma size_tree_eq1 t : (size_ordtree t == 1) = (t == OrdNode [::]).
+Proof.
+case: t => [[| t f]] //=; rewrite eqSS.
+by case: (size_ordtree t) (size_ordtree_pos t).
+Qed.
+Lemma size_bin_to_ordtree bt :
+  size_ordtree (bin_to_ordtree bt) = (size_tree bt).+1.
+Proof.
+elim: bt => [//| l Hl r Hr /=].
+by rewrite add1n -!addnS -!size_ordtreeE {}Hl {}Hr.
+Qed.
+Lemma size_ord_to_bintree t :
+  size_ordtree t = (size_tree (ord_to_bintree t)).+1.
+Proof. by rewrite -size_bin_to_ordtree ord_to_bintreeK. Qed.
+
+
+Section OfSize.
+
+Variable (n : nat).
+
+Structure ordtreesz : predArgType :=
+  OrdTreeSZ {trval :> ordtree; _ : size_ordtree trval == n}.
+HB.instance Definition _ := [isSub of ordtreesz for trval].
+HB.instance Definition _ := [Countable of ordtreesz by <:].
+
+Lemma ordtreeszP (t : ordtreesz) : size_ordtree t = n.
+Proof. by case: t => t /= /eqP. Qed.
+
+End OfSize.
+
+Section FinType.
+
+Implicit Type (t : ordtree).
+
+Definition enum_ordtreesz n :=
+  if n is n'.+1 then [seq bin_to_ordtree b | b <- enum_bintreesz n']
+  else [::].
+
+Lemma size_mem_enum_ordtreeszP n t :
+  t \in enum_ordtreesz n -> size_ordtree t = n.
+Proof.
+case: n => [//| n].
+rewrite -(ord_to_bintreeK t) size_bin_to_ordtree.
+by rewrite (mem_map (can_inj bin_to_ordtreeK)) => /size_mem_enum_bintreeszP ->.
+Qed.
+
+Lemma enum_ordtreeszP n :
+  all (fun t => size_ordtree t == n) (enum_ordtreesz n).
+Proof. by apply/allP => /= t /size_mem_enum_ordtreeszP ->. Qed.
+
+Lemma enum_ordtreesz_uniq n : uniq (enum_ordtreesz n).
+Proof.
+case: n => [// |n].
+rewrite /enum_ordtreesz (map_inj_uniq (can_inj bin_to_ordtreeK)).
+exact: enum_bintreesz_uniq.
+Qed.
+
+Lemma mem_enum_ordtreesz n t :
+  size_ordtree t == n -> t \in enum_ordtreesz n.
+Proof.
+case: n => [/eqP sz0|n].
+  by have := size_ordtree_pos t; rewrite sz0.
+rewrite size_ord_to_bintree eqSS => /mem_enum_bintreesz.
+by move=> /(map_f bin_to_ordtree); rewrite ord_to_bintreeK.
+Qed.
+
+Lemma enum_ordtreesz_countE n t :
+  size_ordtree t == n -> count_mem t (enum_ordtreesz n) = 1.
+Proof.
+move/mem_enum_ordtreesz => H.
+by rewrite (count_uniq_mem _ (enum_ordtreesz_uniq n)) H.
+Qed.
+HB.instance Definition _ n :=
+  Finite.copy (ordtreesz n)
+    (seq_finType (ordtreesz n : subCountType _)
+       (enum_ordtreeszP n) (@enum_ordtreesz_countE n)).
+
+Theorem card_ordtreesz n : #|ordtreesz n.+1| = Catalan_bin n.
+Proof.
+rewrite /= !cardT -!(size_map val) !enumT unlock /=.
+rewrite subType_seqP ?enum_ordtreeszP //= size_map.
+by rewrite size_enum_bintreeszE.
+Qed.
+
+End FinType.
+
+Fixpoint depth_ordtree t :=
+  let: OrdNode f := t in (foldr maxn 0 [seq depth_ordtree t | t <- f]).+1.
+Lemma depth_ordtreeE f :
+  depth_ordtree (OrdNode f) = (foldr maxn 0 [seq depth_ordtree t | t <- f]).+1.
+Proof. by []. Qed.
+Lemma depth_ordtree_pos t : depth_ordtree t > 0.
+Proof. by case: t. Qed.
+Lemma depth_tree_eq1 t : (depth_ordtree t == 1) = (t == OrdNode [::]).
+Proof.
+case: t => [[| t f]] //=; rewrite eqSS.
+case: (depth_ordtree t) (depth_ordtree_pos t) => // n _.
+by case: foldr => // m; rewrite maxnSS.
+Qed.
+Lemma depth_tree_eq2P t :
+  reflect (exists n, t = OrdNode (nseq n.+1 (OrdNode [::])))
+    (depth_ordtree t == 2).
+Proof.
+apply (iffP idP) => [| [n {t}-> /=]]; first last.
+  by rewrite eqSS; elim: n => [//| n /= /eqP ->].
+case: t => f; rewrite [X in X -> _]/= eqSS => /eqP eqmax.
+have /allP alld1 : all (fun t => depth_ordtree t == 1) f.
+  move/eqP : eqmax; rewrite eqn_leq => /andP[+ _].
+  elim: f => [//| t f IHf] /=.
+  rewrite geq_max leq_eqVlt andbC => /andP[{}/IHf -> /orP[-> //|]].
+  by move/(leq_ltn_trans (depth_ordtree_pos t)).
+suff [n eqf] : exists n : nat, f = (nseq n.+1 (OrdNode [::])).
+  by exists n; rewrite eqf.
+exists (size f).-1.
+have {eqmax} -> : (size f).-1.+1 = (size f) by case: f eqmax {alld1}.
+by apply/all_pred1P/allP => /= t {}/alld1; rewrite depth_tree_eq1.
+Qed.
